Start writing compiler correctness theorem
Merely stating the theorem correctly (that is, stating something weak
enough to be true) will be a significant chunk of the work.

src/ConcurrentBridge.v
@@ -1,6 +1,6 @@
 Require Import CoopConcur.
 Require Import ConcurrentCache.
-Require Prog.
+Require Prog Hoare.
 
 Definition valu_conv : valu -> word Prog.Valulen.valulen.
 Proof.
@@ -16,7 +16,7 @@ Proof.
   exact v.
 Defined.
 
-Fixpoint compiler {T} (error_rx: prog Sigma) (p: Prog.prog T)  : prog Sigma :=
+Fixpoint compiler {T} (error_rx: prog Sigma) (p: Prog.prog T) : prog Sigma :=
   match p with
   | Prog.Done v => Done
   | Prog.Read a rx => opt_v <- cache_maybe_read a;
@@ -38,3 +38,70 @@ Fixpoint compiler {T} (error_rx: prog Sigma) (p: Prog.prog T)  : prog Sigma :=
                        compiler error_rx (rx tt)
   | Prog.Trim a rx => compiler error_rx (rx tt)
   end.
+
+Notation prog_valuset := (word Prog.Valulen.valulen * list (word Prog.Valulen.valulen))%type.
+
+(* [lift_disk] and [project_disk] convert between the view of the disk
+from sequential programs [Prog.prog] and concurrent programs [prog]:
+the differences are in the extra state (buffered writes vs race
+detecting readers) and the annoyance of having two different but
+provably equal valu definitions. *)
+
+Definition lift_disk (m: @mem (word Prog.addrlen) _ (const prog_valuset)) : DISK.
+Proof.
+  unfold const in *; intro.
+  destruct (m a); [ apply Some | apply None ].
+  destruct p.
+  exact (valu_conv' w, None).
+Defined.
+
+Definition project_disk (s: abstraction Sigma) : @mem (word Prog.addrlen) _ (const prog_valuset).
+Proof.
+  pose proof (get vDisk0 s) as vd0.
+  unfold const, id in *.
+  intro.
+  destruct (vd0 a); [ apply Some | apply None ].
+  destruct w.
+  exact (valu_conv w, nil).
+Qed.
+
+(* The idea of valid_for_corr2 is to compute a concurrent precondition
+(as part of a Hoare double) corresponding to sequential precondition,
+capturing the same spec on top of the abstraction exported by the
+cache.
+
+Several things are important and currently broken with this
+definition:
+
+- the abstraction from the cache is some combination of vDisk0 and
+  vdisk: vDisk0 is for between system calls and vdisk is for a given
+  system call. [project_disk] currently just uses vDisk0, which is
+  definitely wrong.
+- the precondition needs to copy over the sequential precondition but
+  also add the global invariant and probably state that we aren't in
+  the middle of a system call. This latter condition should be
+  generalized so we can prove valid_for_corr2 about the compiled
+  program by induction.
+*)
+Definition valid_for_corr2 T (pre: Hoare.donecond T ->
+                                   @pred (word Prog.addrlen) _ (const prog_valuset) ->
+                                   @pred (word Prog.addrlen) _ (const prog_valuset)) :
+  (donecond ->
+   DISK -> memory Sigma -> abstraction Sigma -> abstraction Sigma -> Prop) :=
+  fun done d m s0 s =>
+    pre (fun _ d => done (lift_disk d)) (fun _ => False) (project_disk s).
+
+(* The master theorem: convert a sequential program into a concurrent
+program via [compiler], convert its spec to a concurrent spec via
+[valid_for_corr2], and prove the resulting concurrent Hoare double.
+
+Note that a correct [valid_for_corr2] is crucial for starting this
+proof: one nice property is that valid_for_corr2 can separately by
+validated by proving compiler_correct for some specific example
+programs p manually.
+*)
+Theorem compiler_correct : forall T pre R p erx (rx: R -> Prog.prog T) tid,
+    Hoare.corr2 pre (p rx) ->
+    valid delta tid (@valid_for_corr2 T pre) (compiler erx (p rx)).
+Proof.
+Abort.
